theories/config.v
@@ -1,0 +1,49 @@
+Require Import Utf8.
+
+Require Import data_model.
+Require Import prov.
+Require Import relation.
+Require Import types.
+Require Import util.
+
+(*
+  `config` is an inductive type that defines a configuration for the query evaluation.
+  It is either:
+  * `config_error` => An error has occurred.
+  * `config_ok` => The query evaluation is ok. It consists of:
+    - `db` => The database.
+    - `Γ` => The policy environment.
+    - `β` => The privacy budget.
+    - `p` => The provenance context.
+  * `config_output` => The query evaluation is ok and the result is ready to be output. It consists of:
+    - `s` => The schema of the output relation.
+    - `c` => The output configuration.
+*)
+Inductive config: Type :=
+  | config_error: config
+  | config_ok: database → Policy.context → budget → prov_ctx -> config
+  | config_output: relation_wrapped → config → config
+.
+
+Lemma config_output_eq_spec: ∀ r1 r2 c1 c2,
+  config_output r1 c1 = config_output r2 c2 ↔ r1 = r2 ∧ c1 = c2.
+Proof.
+  split; intros.
+  - inversion H. subst. auto.
+  - destruct H. subst. auto.
+Qed.
+
+Definition valid_contexts (Γ: Policy.context) (p: prov_ctx): Prop :=
+  let l1 := List.map fst Γ in
+  let l2 := List.map fst p in
+  sublist _ l1 l2 ∧ sublist _ l2 l1.
+
+Fixpoint config_valid c: Prop :=
+  match c with
+  | config_error => False
+  | config_ok db Γ β p => valid_contexts Γ p
+  | config_output _ c' => config_valid c'
+  end.
+
+Notation "'⟨' db Γ β p '⟩'":= (config_ok db Γ β p)
+  (at level 10, db at next level, Γ at next level, β at next level, p at next level, no associativity).
