theories/tests.v
@@ -1,0 +1,41 @@
+Require Import formula.
+Require Import Utf8.
+
+Section Tests.
+
+Import data_model.
+Import String.
+Import types.
+Import config.
+Import relation.
+Import List.
+
+(* expr = (λ x.x)1 *)
+Example expr :=
+  expression_app
+    (expression_abs ("x"%string) (expression_var "x"%string))
+    (expression_const IntegerType 1).
+
+Example default_config := ⟨ database_empty nil nil nil ⟩.
+Example default_relation := (relation_output nil nil).
+
+Example result_is_1: ∀ env,
+  eval_expr default_config default_relation expr env → snd env = EResultValue IntegerType 1.
+Proof.
+  intros.
+  inversion H. subst. unfold expr in *. simpl in *.
+  inversion H0; subst; intuition; try discriminate.
+
+
+Example relation := (relation_output ((IntegerType, "foo"%string) :: (IntegerType, "bar"%string) :: nil) 
+(((1, 2), (3, 4, tt)) :: nil)).
+(* expr' =  (λ x. _0) 1 *)
+Example expr' := expression_app
+    (expression_abs ("x"%string) (expression_column 0))
+    (expression_const IntegerType 1).
+
+Example result' := snd (eval_expr default_config relation expr').
+Example result'_is_rel : result' = EResultRelation (relation_output ((IntegerType, "foo"%string) :: nil) ((1, 2, tt) :: nil)).
+Proof. reflexivity. Qed.
+
+End Tests.
